\documentclass{article}
\usepackage{epsfig}
\pagestyle{empty}
\begin{document}
\begin{eqnarray*} \tau_{j_1} & = & n_{j_1} ( n_{a_1} \tau_{a_1} + n_{a_2} \tau_{a_2} ) \\[2.5em] \tau_{j_2} & = & n_{j_2} ( n_{a_1} \tau_{a_1} + n_{a_2} \tau_{a_2} ) \end{eqnarray*}
\pagebreak

\begin{eqnarray*} \dot{x}_{j_1} & = & \frac{ \dot{x}_{a_1} / n_{a_1} + \dot{x}_{a_2} / n_{a_2} }{2 n_{j_1}} \\[1em] \dot{x}_{j_2} & = & \frac{ \dot{x}_{a_1} / n_{a_1} - \dot{x}_{a_2} / n_{a_2} }{2 n_{j_2}} \end{eqnarray*}
\pagebreak

\begin{eqnarray*} x_{j_1} & = & \frac{ x_{a_1} / n_{a_1} + x_{a_2} / n_{a_2} }{2 n_{j_1}} + x_{off_1} \\[1em] x_{j_2} & = & \frac{ x_{a_1} / n_{a_1} - x_{a_2} / n_{a_2} }{2 n_{j_1}} + x_{off_2} \end{eqnarray*}
\pagebreak

\begin{eqnarray*} \tau_{a_1} & = & \frac{ \tau_{j_1} / n_{j_1} + \tau_{j_2} / n_{j_2} }{2 n_{a_1}} \\[1em] \tau_{a_2} & = & \frac{ \tau_{j_1} / n_{j_1} - \tau_{j_2} / n_{j_2} }{2 n_{a_1}} \end{eqnarray*}
\pagebreak

\begin{eqnarray*} \dot{x}_{a_1} & = & n_{a_1} ( n_{j_1} \dot{x}_{j_1} + n_{j_2} \dot{x}_{j_2} ) \\[2.5em] \dot{x}_{a_2} & = & n_{a_2} ( n_{j_1} \dot{x}_{j_1} - n_{j_2} \dot{x}_{j_2} ) \end{eqnarray*}
\pagebreak

\begin{eqnarray*} x_{a_1} & = & n_{a_1} \left[ n_{j_1} (x_{j_1} - x_{off_1}) + n_{j_2} (x_{j_2} - x_{off_2}) \right] \\[2.5em] x_{a_2} & = & n_{a_2} \left[ n_{j_1} (x_{j_1} - x_{off_1}) - n_{j_2} (x_{j_2} - x_{off_2}) \right] \end{eqnarray*}
\pagebreak

$ x $
\pagebreak

$ \dot{x} $
\pagebreak

$ \tau $
\pagebreak

$ _a $
\pagebreak

$ _j $
\pagebreak

$ x_{off}$
\pagebreak

$ n $
\pagebreak

$ (0, 1) $
\pagebreak

\begin{eqnarray*} \tau_{j_1} & = & n_{j_1} n_{a_1} \tau_{a_1} \\ \tau_{j_2} & = & n_{j_2} (n_{a_2} \tau_{a_2} - n_{j_1} n_{a_1} \tau_{a_1}) \end{eqnarray*}
\pagebreak

\begin{eqnarray*} \dot{x}_{j_1} & = & \frac{ \dot{x}_{a_1} }{ n_{j_1} n_{a_1} } \\ \dot{x}_{j_2} & = & \frac{ \dot{x}_{a_2} / n_{a_2} - \dot{x}_{a_1} / (n_{j_1} n_{a_1}) }{ n_{j_2} } \end{eqnarray*}
\pagebreak

\begin{eqnarray*} x_{j_1} & = & \frac{ x_{a_1} }{ n_{j_1} n_{a_1} } + x_{off_1} \\ x_{j_2} & = & \frac{ x_{a_2} / n_{a_2} - x_{a_1} / (n_{j_1} n_{a_1}) }{ n_{j_2} } + x_{off_2} \end{eqnarray*}
\pagebreak

\begin{eqnarray*} \tau_{a_1} & = & \tau_{j_1} / (n_{j_1} n_{a_1}) \\ \tau_{a_2} & = & \frac{ \tau_{j_1} + \tau_{j_2} / n_{j_2} }{ n_{a_2} } \end{eqnarray*}
\pagebreak

\begin{eqnarray*} \dot{x}_{a_1} & = & n_{j_1} n_{a_1} \dot{x}_{j_1} \\ \dot{x}_{a_2} & = & n_{a_2} (\dot{x}_{j_1} + n_{j_2} \dot{x}_{j_2}) \end{eqnarray*}
\pagebreak

\begin{eqnarray*} x_{a_1} & = & n_{j_1} n_{a_1} (x_{j_1} - x_{off_1}) \\ x_{a_2} & = & n_{a_2} \left[(x_{j_1} - x_{off_1}) + n_{j_2} (x_{j_2} - x_{off_2})\right] \end{eqnarray*}
\pagebreak

\[ \tau_j = n \tau_a \]
\pagebreak

\[ \dot{x}_j = \dot{x}_a / n \]
\pagebreak

\[ x_j = x_a / n + x_{off} \]
\pagebreak

\[ \tau_a = \tau_j / n\]
\pagebreak

\[ \dot{x}_a = n \dot{x}_j \]
\pagebreak

\[ x_a = n (x_j - x_{off}) \]
\pagebreak

\end{document}
